%\documentclass[11pt]{amsart}
%
%\documentclass[11pt, letterpaper]{article}
%
%\usepackage{amsmath, ulem, graphicx, amsthm, marvosym, multicol}
%\usepackage[left=2cm,right=2cm,top=2cm,bottom=2cm]{geometry}
%
%\renewcommand{\familydefault}{\sfdefault}
%
%%\usepackage{graphics}
%
%%\topmargin -.5in
%%\evensidemargin-.1in
%%\oddsidemargin-.1in
%%\textheight 9in
%%\textwidth 6.5in
%
%\newtheorem*{definition}{Definition}
%%\setlength{\voffset}{-1in}
%
%\everymath={\displaystyle}
%
%%%% 
%% Framed mini-page environment 
%%%%
%\newsavebox{\fmbox}
%   \newenvironment{ans}
%     {\begin{lrbox}{\fmbox}\begin{minipage}{13cm} \textbf{Answer:} \par}
%     {\end{minipage}\end{lrbox}\fbox{\usebox{\fmbox}} \vspace{0.25cm}}
%
%\newcommand{\lcm}{\operatorname{lcm}}
%\newcommand{\ds}{\displaystyle}
%
%\newcommand{\lilspa}{\vspace{.15in}}
%
%\begin{document}

\pagestyle{empty}


%\begin{center}
%{\sc  {\large Taylor Series Summary Sheet}\\
%Math 1336 \& 1337  (Dr. Christine Cole)
%%\\May 16, 2014
%}
%\end{center}
%
%\vspace*{.1in}

{\sc Definition for Taylor Series for \(f(x)\) centered at \(a\):}
%\vspace*{-.1in}
\begin{eqnarray*}
\sum_{n=0}^\infty \frac{f^{(n)}(a)}{n!}(x-a)^n &=& f(a) + f^{(1)}(a)(x-a) + \frac{f^{(2)}(a)}{2!}(x-a)^2\\
&& +\ \frac{f^{(3)}(a)}{3!}(x-a)^3+\frac{f^{(4)}(a)}{4!}(x-a)^4+\ldots\\
\end{eqnarray*}

%\vspace*{.1in}

{\sc Definition for Maclaurin Series for \(f(x)\):}
%\vspace*{-.1in}
\begin{eqnarray*}
\sum_{n=0}^\infty \frac{f^{(n)}(0)}{n!}x^n &=& f(0) + f^{(1)}(0)x 
+ \frac{f^{(2)}(0)}{2!}x^2 + \frac{f^{(3)}(0)}{3!}x^3+\frac{f^{(4)}(0)}{4!}x^4+\ldots\\
\end{eqnarray*}

%\vspace*{-.2in}
%\begin{framed}
{\sc Taylor's Formula / Lagrange's Form of the Remainder:}

%\vspace*{-.1in}
\begin{eqnarray*}
R_n(x) = \frac{f^{(n+1)}(z)}{(n+1)!}(x-a)^{n+1}, \qquad \qquad %\textbf{Will NOT be covered in Spring 2024}
\end{eqnarray*}
%\vspace*{-.2in}
%\end{framed}


%\vspace*{.1in}

{\sc Alternating Series Estimation Theorem Formula:}
%\vspace*{-.1in}
\begin{eqnarray*}
|R_N| = \left| S - S_N \right | \leq b_{N+1}
\end{eqnarray*}



\vspace*{.1in}

%
%{\sc Taylor's Formula / Lagrange's Form of the Remainder:}
%
%\vspace*{-.1in}
%\begin{eqnarray*}
%R_n(x) = \frac{f^{(n+1)}(z)}{(n+1)!}(x-a)^{n+1}
%\end{eqnarray*}
%
%
%
%%\vspace*{.1in}
%
%{\sc Alternating Series Estimation Theorem Formula:}
%\vspace*{-.1in}
%\begin{eqnarray*}
%|R_n| = \left| S - S_n \right | \leq b_{n+1}
%\end{eqnarray*}
%
%
%
%\vspace*{.1in}


{\sc Selected Maclaurin Series with Radius of Convergence, \(R\):}

\begin{eqnarray*}
e^x = \sum_{n=0}^\infty \frac{x^n}{n!} &=& 1+x+\frac{x^2}{2!}+\frac{x^3}{3!}+\frac{x^4}{4!}+\ldots, \quad R=\infty\\
&&\\
&&\\
\sin(x) = \sum_{n=0}^\infty \frac{(-1)^n x^{2n+1}}{(2n+1)!} &=& x-\frac{x^3}{3!}+\frac{x^5}{5!}-\frac{x^7}{7!}+\frac{x^9}{9!}-\ldots, \quad R=\infty\\
&&\\
&&\\
\cos(x) = \sum_{n=0}^\infty \frac{(-1)^n x^{2n}}{(2n)!} &=& 1-\frac{x^2}{2!}+\frac{x^4}{4!}-\frac{x^6}{6!}+\frac{x^8}{8!}-\ldots, \quad R=\infty\\
&&\\
&&\\
\mathrm{Geometric\ Series:\ } \frac{1}{1-x} = \sum_{n=0}^\infty x^{n} &=& 1+x+x^2+x^3+x^4+\ldots, \quad R=1\\
&&\\
&&\\
\ln(1+x) = \sum_{n=1}^\infty \frac{(-1)^{n+1} x^n}{n} &=& x-\frac{x^2}{2}+\frac{x^3}{3}-\frac{x^4}{4}+\frac{x^5}{5}-\ldots, \quad R=1\\
%&&\\
%&&\\
%\mathrm{Binomial\ Series:\ } (1+x)^k = \sum_{n=0}^\infty\begin{pmatrix} k\\n \end{pmatrix} x^{n} &=& 1+kx+\frac{k(k-1)}{2!}x^2+\frac{k(k-1)(k-2)}{3!}x^3+\ldots, \quad R=1\\
\end{eqnarray*}
%\end{document}
